QI_Checker/IR/Ctx.lean
@@ -1,1 +1,0 @@
-import QI_Checker.IR.TermType
