QI_Checker/Instantiation/subst.lean
@@ -1,0 +1,105 @@
+import QI_Checker.IR.TermType
+import QI_Checker.IR.Term
+import QI_Checker.IR.Op
+
+open IR
+
+/-- Append an element to a substitution or a renaming.
+```
+Δ ⊢ σ : Γ  Γ ⊢ A  Δ ⊢ t : A[σ]
+------------------------------
+Δ ⊢ σ.t : Γ.A
+``` -/
+def snoc.{u} {X : Sort u} (σ : Nat → X) (x : X) : Nat → X
+  | 0   => x
+  | n+1 => σ n
+
+@[simp]
+theorem snoc_zero {X} (σ : Nat → X) (x : X) : snoc σ x 0 = x := rfl
+
+@[simp]
+theorem snoc_succ {X} (σ : Nat → X) (x : X) (n) : snoc σ x (n + 1) = σ n := rfl
+
+/-! ## Renaming -/
+
+
+/-- Lift a renaming under a binder 1 time. See `up`. -/
+def upr (ξ : Nat → Nat) : Nat → Nat :=
+  snoc (fun i => ξ i + 1) 0
+
+
+@[simp]
+theorem upr_id : upr id = id := by
+  ext ⟨⟩ <;> dsimp [upr, snoc]
+
+/-- Rename the de Bruijn indices in an expression. -/
+def rename (ξ : Nat → Nat) : Term → Term :=
+  sorry
+
+/-! ## Substitution -/
+
+/-- Lift a substitution under a binder.
+```
+Δ ⊢ σ : Γ  Γ ⊢ A
+------------------------
+Δ.A[σ] ⊢ (↑≫σ).v₀ : Γ.A
+```
+
+Warning: don't unfold this definition! Use `up_eq_snoc` instead. -/
+@[irreducible]
+def up (σ : Nat → Term) : Nat → Term :=
+  snoc (rename Nat.succ ∘ σ) (.var 0)
+
+
+@[simp]
+theorem up_var : up Term.var = Term.var := by
+  ext ⟨⟩ <;> (unfold up; dsimp [snoc, rename]); sorry
+
+/-- Apply a substitution to a term. -/
+def subst (σ : Nat → Term) : Term → Term := sorry
+
+
+@[simp]
+theorem subst_bvar: subst Term.var = id := by sorry
+  --ext t; dsimp; induction t <;> grind [subst, up_bvar]
+
+@[simp]
+theorem subst_snoc_zero (σ : Nat → Term) (t : Term) : subst (snoc σ t) (.var 0) = t := by
+  dsimp [subst, snoc]; sorry
+
+/-- Turn a renaming into a substitution. -/
+def ofRen (ξ : Nat → Nat) : Nat → Term :=
+  fun i => Term.var (ξ i)
+
+@[simp]
+theorem ofRen_id : ofRen id = Term.var := rfl
+
+theorem ofRen_upr: ofRen (upr ξ) = up (ofRen ξ) := by
+  ext ⟨⟩ <;> simp [ofRen, upr, up, snoc, rename]; sorry
+
+theorem rename_eq_subst_ofRen (ξ : Nat → Nat) : rename ξ = subst (ofRen ξ) := by sorry
+  -- ext t
+  -- induction t generalizing ξ <;> dsimp [rename, subst]
+  -- case bvar => simp [ofRen]
+  -- all_goals grind [ofRen_upr]
+
+/-- Compose two substitutions.
+```
+Θ ⊢ σ : Δ  Δ ⊢ τ : Γ
+--------------------
+Θ ⊢ σ≫τ : Γ
+``` -/
+def comp (σ τ : Nat → Term) : Nat → Term :=
+  subst σ ∘ τ
+
+@[simp]
+theorem bvar_comp (σ : Nat → Term) : comp Term.var σ = σ := by
+  ext i; simp [comp]
+
+@[simp]
+theorem comp_bvar (σ : Nat → Term) : comp σ Term.var = σ := by
+  ext i; simp [comp, subst]; sorry
+
+theorem up_comp_ren_sb (ξ : Nat → Nat) (σ : Nat → Term) :
+    up (σ ∘ ξ) = up σ ∘ upr ξ := by
+  ext ⟨⟩ <;> (unfold up; dsimp [snoc, upr])
